lib/zoo_std/inf_array.ml
@@ -9,25 +9,27 @@ let create default =
   let mutex = Mutex.create () in
   { data; default; mutex }
 
+let next_capacity n =
+  Int.max 8 (if n <= 512 then 2 * n else n + n / 2)
+let reserve t n =
+  let data = t.data in
+  let cap = Array.size data in
+  if cap < n then (
+    let cap = Int.max n (next_capacity cap) in
+    let data = Array.unsafe_grow data cap t.default in
+    t.data <- data
+  )
+
 let get t i =
-  Mutex.protect t.mutex (fun () ->
+  Mutex.protect t.mutex @@ fun () ->
     let data = t.data in
     if i < Array.size data then (
       Array.unsafe_get data i
     ) else (
       t.default
     )
-  )
 
 let set t i v =
-  Mutex.protect t.mutex (fun () ->
-    let data = t.data in
-    let sz = Array.size data in
-    if i < sz then (
-      Array.unsafe_set data i v
-    ) else (
-      let data = Array.unsafe_grow data (Int.max (i + 1) (2 * sz)) t.default in
-      Array.unsafe_set data i v ;
-      t.data <- data
-    )
-  )
+  Mutex.protect t.mutex @@ fun () ->
+    reserve t (i + 1) ;
+    Array.unsafe_set t.data i v
