theories/zoo_std/inf_array.v
@@ -75,19 +75,22 @@ Section inf_array_G.
   #[local] Definition inf_array_model₂ γ vs :=
     inf_array_model₂' γ.(inf_array_meta_model) vs.
 
-  #[local] Definition inf_array_inv_inner l γ : iProp Σ :=
-    ∃ data us vs,
+  #[local] Definition inf_array_inv'' l γ us : iProp Σ :=
+    ∃ data vs,
     l.[data] ↦ data ∗
     array_model data (DfracOwn 1) us ∗
     inf_array_model₂ γ vs ∗
     ⌜vs = λ i, if decide (i < length us) then us !!! i else γ.(inf_array_meta_default)⌝.
+  #[local] Definition inf_array_inv' l γ : iProp Σ :=
+    ∃ us,
+    inf_array_inv'' l γ us.
   Definition inf_array_inv t : iProp Σ :=
     ∃ l γ mtx,
     ⌜t = #l⌝ ∗
     meta l nroot γ ∗
     l.[default] ↦□ γ.(inf_array_meta_default) ∗
     l.[mutex] ↦□ mtx ∗
-    mutex_inv mtx (inf_array_inv_inner l γ).
+    mutex_inv mtx (inf_array_inv' l γ).
 
   Definition inf_array_model t vs : iProp Σ :=
     ∃ l γ,
@@ -208,10 +211,10 @@ Section inf_array_G.
     iIntros "%Φ _ HΦ".
 
     wp_rec.
-    wp_apply (array_create_spec with "[//]") as "%data Hmodel_data".
+    wp_apply (array_create_spec with "[//]") as "%data Hdata".
     wp_smart_apply (mutex_create_spec_init with "[//]") as (mtx) "Hmtx_init".
-    wp_block l as "Hmeta" "(Hdata & Hdefault & Hmtx & _)".
-    iMod (pointsto_persist with "Hdefault") as "#Hdefault".
+    wp_block l as "Hmeta" "(Hl_data & Hl_default & Hl_mtx & _)".
+    iMod (pointsto_persist with "Hl_default") as "#Hl_default".
 
     iMod (inf_array_model_alloc default) as "(%γ_model & Hmodel₁ & Hmodel₂)".
 
@@ -221,8 +224,56 @@ Section inf_array_G.
     |}.
     iMod (meta_set _ _ γ with "Hmeta") as "#Hmeta"; first done.
 
-    iMod (mutex_init_to_inv (inf_array_inv_inner l γ) with "Hmtx_init [Hdata Hmodel_data Hmodel₂]") as "#Hmtx_inv"; first iSteps.
+    iMod (mutex_init_to_inv (inf_array_inv' l γ) with "Hmtx_init [Hl_data Hdata Hmodel₂]") as "#Hmtx_inv".
+    { rewrite /inf_array_inv'. iSteps. }
     iSteps.
+  Qed.
+
+  #[local] Lemma inf_array_next_capacity_spec n :
+    (0 ≤ n)%Z →
+    {{{
+      True
+    }}}
+      inf_array_next_capacity #n
+    {{{ m,
+      RET #m;
+      ⌜n ≤ m⌝%Z
+    }}}.
+  Proof.
+    iSteps; iModIntro; wp_apply maximum_spec; iSteps.
+  Qed.
+  #[local] Lemma inf_array_reserve_spec l γ us n :
+    (0 ≤ n)%Z →
+    {{{
+      l.[default] ↦□ γ.(inf_array_meta_default) ∗
+      inf_array_inv'' l γ us
+    }}}
+      inf_array_reserve #l #n
+    {{{ us,
+      RET ();
+      inf_array_inv'' l γ us ∗
+      ⌜Z.to_nat n ≤ length us⌝
+    }}}.
+  Proof.
+    iIntros "%Hn %Φ (#Hl_default & (%data & %vs & Hl_data & Hdata & Hmodel₂ & %Hvs)) HΦ".
+
+    wp_rec. wp_load.
+    wp_smart_apply (array_size_spec with "Hdata") as "Hdata".
+    wp_pures. case_bool_decide; last iSteps.
+    wp_smart_apply (inf_array_next_capacity_spec with "[//]") as (?) "%"; first lia.
+    wp_apply maximum_spec.
+    wp_load.
+    wp_smart_apply (array_unsafe_grow_spec with "Hdata") as (data') "(Hdata & Hdata')"; first lia.
+    wp_store.
+
+    iSteps; iPureIntro; rewrite length_app length_replicate; last lia.
+    apply functional_extensionality => i. rewrite Hvs.
+    case_decide; last case_decide.
+    - rewrite decide_True; first lia.
+      rewrite lookup_total_app_l //.
+    - rewrite lookup_total_app_r; first lia.
+      rewrite lookup_total_replicate_2 //; first lia.
+    - done.
   Qed.
 
   Lemma inf_array_get_spec t i :
@@ -239,18 +290,18 @@ Section inf_array_G.
       True
     >>>.
   Proof.
-    iIntros "% !> %Φ (%l & %γ & %mtx & -> & #Hmeta & #Hmtx & #Hdefault & #Hinv_mtx) HΦ".
+    iIntros "% !> %Φ (%l & %γ & %mtx & -> & #Hmeta & #Hl_mtx & #Hl_default & #Hmtx_inv) HΦ".
     Z_to_nat i. rewrite Nat2Z.id.
 
     wp_rec. wp_load.
-    wp_apply (mutex_protect_spec Φ with "[$Hinv_mtx HΦ]"); last iSteps. iIntros "Hlocked_mtx (%data & %us & %vs & Hdata & Hmodel_data & Hmodel₂ & %Hvs)".
+    wp_apply (mutex_protect_spec Φ with "[$Hmtx_inv HΦ]"); last iSteps. iIntros "Hmtx_locked (%us & %data & %vs & Hl_data & Hdata & Hmodel₂ & %Hvs)".
     wp_load.
-    wp_smart_apply (array_size_spec with "Hmodel_data") as "Hmodel_data".
+    wp_smart_apply (array_size_spec with "Hdata") as "Hdata".
     wp_pures. case_decide.
 
     - rewrite bool_decide_eq_true_2; first lia.
       iApply wp_fupd.
-      wp_smart_apply (array_unsafe_get_spec with "Hmodel_data"); [done | | done |].
+      wp_smart_apply (array_unsafe_get_spec with "Hdata"); [done | | done |].
       { rewrite Nat2Z.id list_lookup_lookup_total_lt //. lia. }
 
       iMod "HΦ" as "(%_vs & (%_l & %_γ & %Heq & #_Hmeta & Hmodel₁) & _ & HΦ)". injection Heq as <-.
@@ -258,7 +309,8 @@ Section inf_array_G.
       iDestruct (inf_array_model_agree with "Hmodel₁ Hmodel₂") as %->.
       iMod ("HΦ" with "[Hmodel₁]") as "HΦ"; first iSteps.
 
-      iSteps. rewrite Hvs decide_True; first lia. iSteps.
+      rewrite /inf_array_inv'. iSteps.
+      rewrite Hvs decide_True; first lia. iSteps.
 
     - rewrite bool_decide_eq_false_2; first lia. wp_load.
 
@@ -267,6 +319,7 @@ Section inf_array_G.
       iDestruct (inf_array_model_agree with "Hmodel₁ Hmodel₂") as %->.
       iMod ("HΦ" with "[Hmodel₁]") as "HΦ"; first iSteps.
 
+      rewrite /inf_array_inv'. iSteps.
       rewrite Hvs decide_False; first lia. iSteps.
   Qed.
   Lemma inf_array_get_spec' t i :
@@ -305,74 +358,32 @@ Section inf_array_G.
       True
     >>>.
   Proof.
-    iIntros "% !> %Φ (%l & %γ & %mtx & -> & #Hmeta & #Hmtx & #Hdefault & #Hinv_mtx) HΦ".
+    iIntros "% !> %Φ (%l & %γ & %mtx & -> & #Hmeta & #Hl_mtx & #Hl_default & #Hmtx_inv) HΦ".
     Z_to_nat i. rewrite Nat2Z.id.
 
     wp_rec. wp_load.
-    wp_apply (mutex_protect_spec Φ with "[$Hinv_mtx HΦ]"); last iSteps. iIntros "Hlocked_mtx (%data & %us & %vs & Hdata & Hmodel_data & Hmodel₂ & %Hvs)".
+    wp_apply (mutex_protect_spec Φ with "[$Hmtx_inv HΦ]"); last iSteps. iIntros "Hmtx_locked (%us & Hinv)".
+    wp_smart_apply (inf_array_reserve_spec with "[$]") as "{%} %us ((%data & %vs & Hl_data & Hdata & Hmodel₂ & %Hvs) & %)"; first lia.
     wp_load.
-    wp_smart_apply (array_size_spec with "Hmodel_data") as "Hmodel_data".
-    wp_pures. case_decide.
+    iApply wp_fupd.
+    wp_smart_apply (array_unsafe_set_spec with "Hdata") as "Hdata"; first lia.
 
-    - rewrite bool_decide_eq_true_2; first lia.
-      iApply wp_fupd.
-      wp_smart_apply (array_unsafe_set_spec with "Hmodel_data") as "Hmodel_data"; first done.
+    iMod "HΦ" as "(%_vs & (%_l & %_γ & %Heq & #_Hmeta & Hmodel₁) & _ & HΦ)". injection Heq as <-.
+    iDestruct (meta_agree with "Hmeta _Hmeta") as %<-. iClear "_Hmeta".
+    iDestruct (inf_array_model_agree with "Hmodel₁ Hmodel₂") as %->.
+    set us' := <[i := v]> us.
+    set vs' := <[i := v]> vs.
+    iMod (inf_array_model_update vs' with "Hmodel₁ Hmodel₂") as "(Hmodel₁ & Hmodel₂)".
+    iMod ("HΦ" with "[Hmodel₁]") as "HΦ"; first iSteps.
 
-      iMod "HΦ" as "(%_vs & (%_l & %_γ & %Heq & #_Hmeta & Hmodel₁) & _ & HΦ)". injection Heq as <-.
-      iDestruct (meta_agree with "Hmeta _Hmeta") as %<-. iClear "_Hmeta".
-      iDestruct (inf_array_model_agree with "Hmodel₁ Hmodel₂") as %->.
-      set us' := <[i := v]> us.
-      set vs' := <[i := v]> vs.
-      iMod (inf_array_model_update vs' with "Hmodel₁ Hmodel₂") as "(Hmodel₁ & Hmodel₂)".
-      iMod ("HΦ" with "[Hmodel₁]") as "HΦ"; first iSteps.
-
-      iFrame. iSplitR "HΦ"; last iSteps. iPureIntro.
-      rewrite Nat2Z.id /us' /vs' length_insert Hvs.
-      apply functional_extensionality => j. destruct (decide (j = i)) as [-> |].
-      + rewrite fn_lookup_insert decide_True; first lia.
-        rewrite list_lookup_total_insert //. lia.
-      + rewrite fn_lookup_insert_ne //. case_decide; last done.
-        rewrite list_lookup_total_insert_ne //.
-
-    - rewrite bool_decide_eq_false_2; first lia. wp_load.
-      wp_smart_apply maximum_spec.
-      wp_smart_apply (array_unsafe_grow_spec with "Hmodel_data") as "%data' Hmodel_data'"; first lia.
-      wp_smart_apply (array_unsafe_set_spec with "Hmodel_data'") as "Hmodel_data'".
-      { rewrite length_app length_replicate. lia. }
-      rewrite Nat2Z.id insert_app_r_alt; first lia.
-      rewrite insert_replicate_lt; first lia.
-      rewrite -Nat.sub_succ_l; first lia.
-      wp_store.
-
-      iMod "HΦ" as "(%_vs & (%_l & %_γ & %Heq & #_Hmeta & Hmodel₁) & _ & HΦ)". injection Heq as <-.
-      iDestruct (meta_agree with "Hmeta _Hmeta") as %<-. iClear "_Hmeta".
-      iDestruct (inf_array_model_agree with "Hmodel₁ Hmodel₂") as %->.
-      set us' := us ++ _.
-      set vs' := <[i := v]> vs.
-      iMod (inf_array_model_update vs' with "Hmodel₁ Hmodel₂") as "(Hmodel₁ & Hmodel₂)".
-      iMod ("HΦ" with "[Hmodel₁]") as "HΦ"; first iSteps.
-
-      iModIntro. iFrame. iSplitR "HΦ"; last iSteps. iPureIntro.
-      rewrite /us' /vs' !length_app length_replicate Hvs /=.
-      apply functional_extensionality => j. destruct (Nat.lt_total j i) as [| [-> |]].
-      + rewrite fn_lookup_insert_ne; first lia.
-        rewrite (@decide_True _ (j < _ + _)); first lia.
-        case_decide.
-        * rewrite lookup_total_app_l //.
-        * rewrite lookup_total_app_r; first lia.
-          rewrite lookup_total_app_l; first (rewrite length_replicate //; lia).
-          rewrite lookup_total_replicate_2 //. lia.
-      + rewrite fn_lookup_insert decide_True; first lia.
-        rewrite lookup_total_app_r; first lia.
-        rewrite lookup_total_app_r length_replicate; first lia.
-        rewrite Nat.sub_diag //.
-      + rewrite length_replicate fn_lookup_insert_ne; first lia.
-        rewrite decide_False; first lia.
-        case_decide; last done.
-        rewrite lookup_total_app_r; first lia.
-        rewrite lookup_total_app_r length_replicate; first lia.
-        rewrite lookup_total_cons_ne_0; first lia.
-        rewrite lookup_total_replicate_2 //; first lia.
+    iFrame. iSplitR "HΦ"; last iSteps. iPureIntro.
+    rewrite Nat2Z.id /us' /vs' length_insert Hvs.
+    apply functional_extensionality => j.
+    destruct (decide (j = i)) as [-> |].
+    - rewrite fn_lookup_insert decide_True; first lia.
+      rewrite list_lookup_total_insert //. lia.
+    - rewrite fn_lookup_insert_ne //. case_decide; last done.
+      rewrite list_lookup_total_insert_ne //.
   Qed.
   Lemma inf_array_set_spec' t i v :
     (0 ≤ i)%Z →
